$$
\frac{7}{x+8} = \frac{6}{2-x}
$$
$$
7 * (2-x)=6*(x+8)
$$
$$
7*2-7x=6x+6*8
$$
$$
7*2-7x-6x=6*8
$$
$$
7*2-(7x+6x)=6*8
$$
$$
14-13x=48
$$
$$
13x = 14-48 = -34
$$
$$
x = \frac{-34}{13} = -\frac{-34}{13}
$$
---
$$
\frac{7}{-\frac{34}{13} + 8} = \frac{6}{2 - -\frac{34}{13}}
$$
$$
\frac{7}{-2\frac{8}{13}+8}=\frac{6}{2+2\frac{8}{13}}
$$
$$
\frac{7}{6\frac{8}{13}}=\frac{6}{4\frac{8}{13}}
$$
---
$$
7:6\frac{8}{13}=\frac{7}{1}:\frac{86}{13}=\frac{7 * 13}{1 * 86}=\frac{91}{86}=1\frac{15}{86}
$$
$$
6:4\frac{8}{13}=\frac{6}{1}:\frac{60}{13}=\frac{6*13}{1*60}=\frac{78}{60}=\frac{39}{30}=13
$$