#math #homework

$$2(x+2)-3(x-2)=5-4(3x-1)$$
$$2x+2*2-3x+3*2=5-4*3x+4*1$$
$$
2x+4-3x+6=5-12x+4
$$
$$
-1x+10=9-12x
$$
$$
-1x+10-9+12x=0
$$
$$
11x+1=0
$$
$$
11x=0-1=-1
$$
$$
x=-1:11=-\frac{1}{11}
$$
---
$$
2(-\frac{1}{11}+2)-3(-\frac{1}{11}-2)=5-4(3*-\frac{1}{11}-1)
$$
$$
2*-\frac{1}{11}+2*2-3*-\frac{1}{11}+3*2=5-4*3*-\frac{1}{11}+4*1
$$
$$
2*-\frac{1}{11}+4-3*-\frac{1}{11}+6=5-12*-\frac{1}{11}+4
$$
$$
\frac{1}{11}+10=9+\frac{12}{11}
$$
$$
10\frac{1}{11}=9+1\frac{1}{11}
$$
$$
10\frac{1}{11}=10\frac{1}{11}
$$
